code/experimental/pkcs/Hacl.Impl.PKCS11.Creation.GenKey.fst
@@ -3,6 +3,7 @@ module Hacl.Impl.PKCS11.Creation.GenKey
 open Hacl.Impl.PKCS11.Internal.Types
 open Hacl.Impl.PKCS11.Internal.Attribute
 open Hacl.Impl.PKCS11.DeviceModule
+open Hacl.Impl.PKCS11.Session
 
 open Hacl.Impl.PKCS11.Result
 
@@ -30,29 +31,40 @@ The object created by a successful call to C_GenerateKey will have its CKA_LOCAL
 
 Return values: CKR_ARGUMENTS_BAD, 
 CKR_ATTRIBUTE_READ_ONLY -> val isAttributeReadOnly: _CK_ATTRIBUTE_TYPE -> Tot (r: exception_t {CKR_OK? r \/ CKR_ATTRIBUTE_READ_ONLY? r})
-CKR_ATTRIBUTE_TYPE_INVALID - impossible to create an invalid type, only if parsing? 
-
-
-CKR_ATTRIBUTE_VALUE_INVALID, CKR_CRYPTOKI_NOT_INITIALIZED, CKR_CURVE_NOT_SUPPORTED, CKR_DEVICE_ERROR, CKR_DEVICE_MEMORY, CKR_DEVICE_REMOVED, CKR_FUNCTION_CANCELED, CKR_FUNCTION_FAILED, CKR_GENERAL_ERROR, CKR_HOST_MEMORY, CKR_MECHANISM_INVALID, CKR_MECHANISM_PARAM_INVALID, CKR_OK, CKR_OPERATION_ACTIVE, CKR_PIN_EXPIRED, CKR_SESSION_CLOSED, CKR_SESSION_HANDLE_INVALID, CKR_SESSION_READ_ONLY, CKR_TEMPLATE_INCOMPLETE, CKR_TEMPLATE_INCONSISTENT, CKR_TOKEN_WRITE_PROTECTED, CKR_USER_NOT_LOGGED_IN.
+CKR_ATTRIBUTE_TYPE_INVALID - see parsing
+CKR_ATTRIBUTE_VALUE_INVALID - see parsing
+CKR_CRYPTOKI_NOT_INITIALIZED, CKR_CURVE_NOT_SUPPORTED, CKR_DEVICE_ERROR, CKR_DEVICE_MEMORY, CKR_DEVICE_REMOVED, CKR_FUNCTION_CANCELED, CKR_FUNCTION_FAILED, CKR_GENERAL_ERROR, CKR_HOST_MEMORY, CKR_MECHANISM_INVALID, CKR_MECHANISM_PARAM_INVALID, CKR_OK, CKR_OPERATION_ACTIVE, CKR_PIN_EXPIRED, CKR_SESSION_CLOSED, CKR_SESSION_HANDLE_INVALID, CKR_SESSION_READ_ONLY, CKR_TEMPLATE_INCOMPLETE, CKR_TEMPLATE_INCONSISTENT, CKR_TOKEN_WRITE_PROTECTED, CKR_USER_NOT_LOGGED_IN.
 
 *)
 
 
 val _CKS_GenerateKey: 
+  #t: Type0 -> 
   d: device -> 
-  hSession: _CK_SESSION_HANDLE ->
+  hSession: _CK_SESSION_HANDLE -> 
+  pMechanism: _CK_MECHANISM_TYPE -> 
+  ulCount: size_t -> 
+  pTemplate: buffer (attributeD #t) {length pTemplate = uint_v ulCount} -> 
+  Stack 
+    (exception_t & _CK_OBJECT_HANDLE)
+  (requires fun h -> True)
+  (ensures fun h0 _ h1 -> True)
+
+
+
+
+val _CKS_GenerateKey_: 
+  d: device -> 
+  hSession: _CK_SESSION_HANDLE {getDeviceInitialised d hSession} ->
   pMechanism: _CK_MECHANISM_TYPE ->
   ulCount: size_t -> 
   pTemplate: buffer attribute {length pTemplate = uint_v ulCount} -> 
-  test: attributeD #uint32 -> 
   Stack 
     ((handler: result nat) & (device))
     (requires fun h -> True)
     (ensures fun h0 _ h1 -> True)
 
-open Hacl.Impl.PKCS11.Parsing 
-
-let _CKS_GenerateKey d hSession pMechanism ulCould pTemplate test = 
+let _CKS_GenerateKey_ d hSession pMechanism ulCould pTemplate = 
   let testCall = checkAttributes ulCould pTemplate in 
 
   (|Inl 0, d|) 
