code/experimental/pkcs/Hacl.Impl.PKCS11.Parsing.fst
@@ -10,6 +10,8 @@ open Hacl.Impl.PKCS11.Internal.Attribute
 open Hacl.Impl.PKCS11.Internal.Types
 open Hacl.Impl.PKCS11.Result
 
+open LowStar.Buffer
+
 (* totally wrong, i know, just an example.
 The idealistic is to check whether it is void or not, then to check whether they between each other are equal. I have no idea how to do it for now, so. 
 *)
@@ -18,33 +20,31 @@ The idealistic is to check whether it is void or not, then to check whether they
   Exceptions: 
   CKR_ATTRIBUTE_TYPE_INVALID -> in parsing the main match to have a value out of possible
   CKR_ATTRIBUTE_VALUE_INVALID -> in the second match if the checkes are not satisfied (i.e. can't cast to the attribute)
+
+
+NB: I am NOT sure that this code is critical to the work itself, it's more about intercommunication.
+
+
 *)
 
 
-val compareT: t0: Type0 -> t1: Type0 -> Tot bool
+(*
+  For the eq types -> if eq t0 t1 then true
+  For not eq types -> if t0 == t1 (i.e. the same type), even if by hand
 
-let compareT t0 t1 = 
-  match t0 with 
-  |void -> match t1 with |void -> true |_ -> false
-  |_ -> false
-  
+*)
+assume val compareT: t0: Type0 -> t1: Type0 -> Tot (t: bool {t0 == t1})
 
-val parseAttribute: #t: Type0 -> attributeD #t -> 
-  Stack (result attribute)
+
+assume val parseAttribute: #t: Type0 -> a: attributeD #t -> 
+  StackInline (exception_t & attribute)
   (requires fun h -> True)
   (ensures fun h0 _ h1 -> True)
 
-let parseAttribute #t a = 
-  let attrT = uint_v (a._type) in 
-  match attrT with 
-  | 0 -> 
-    let expectedType = void_t (typeID_type attrT) in 
-    let expectedLen = lenAttribute a._type in 
-    if not (compareT expectedType t) then 
-      Inr CKR_ARGUMENTS_BAD
-    else if not (eq expectedLen a.ulValueLen) then
-      Inr CKR_ARGUMENTS_BAD
-    else  
-      Inl (CKA_CLASS a._type  a.pValue a.ulValueLen)
-  | _ -> Inr CKR_ARGUMENTS_BAD
-    
+assume val parseAttributes: #t: Type0 -> ulCount: size_t -> pTemplate: buffer (attributeD #t)  {length pTemplate = uint_v ulCount} -> 
+  StackInline 
+    (e: exception_t 
+      {CKR_ATTRIBUTE_TYPE_INVALID? e \/ CKR_ATTRIBUTE_VALUE_INVALID? e \/ CKR_ARGUMENTS_BAD? e} & buffer attribute)
+  (requires fun h -> live h pTemplate)
+  (ensures fun h0 _ h1 -> True)
+
