code/experimental/pkcs/Hacl.Impl.PKCS11.Session.fst
@@ -1,0 +1,6 @@
+module Hacl.Impl.PKCS11.Session
+
+open Hacl.Impl.PKCS11.Internal.Types
+open Hacl.Impl.PKCS11.DeviceModule
+
+assume val getDeviceInitialised: d: device -> hSession: _CK_SESSION_HANDLE -> Tot bool
